yalla/mll_pn_to_seq_parr.v
@@ -35,6 +35,276 @@ Notation switching := (@switching atom).
 Notation switching_left := (@switching_left atom).
 
 
+Section Rem_node.
+Context {G : proof_structure} {v : G}.
+Hypothesis (V : vlabel v = ⊗ \/ vlabel v = ⅋) (T : terminal v).
+
+(* Vertices neighbourhing v *)
+Local Notation elv := (left V).
+Local Notation erv := (right V).
+Local Notation ecv := (ccl V).
+Local Notation lv := (source elv).
+Local Notation rv := (source erv).
+Local Notation cv := (target ecv).
+
+(** Base graph for removing a node and its eventual conclusion *) (* TODO faire comme add_node des cas selon vlabel_v pour factoriser ? *)
+Definition rem_node_graph_1 := induced ([set: G] :\ v :\ cv).
+
+(* Then add new conclusions *)
+Lemma lv_inside : lv \in setT :\ v :\ cv.
+Proof.
+  rewrite !in_set !in_set1. splitb; apply /eqP => F.
+  - assert (P : walk lv lv [:: elv ; ecv]) by by rewrite /= F ccl_e left_e; splitb.
+    by specialize (ps_acyclic P).
+  - assert (FF : lv = target elv) by by rewrite left_e.
+    apply (no_selfloop FF).
+Qed.
+
+Lemma rv_inside : rv \in setT :\ v :\ cv.
+Proof.
+  rewrite !in_set !in_set1. splitb; apply /eqP => F.
+  - assert (P : walk rv rv [:: erv ; ecv]) by by rewrite /= F ccl_e right_e; splitb.
+    by specialize (ps_acyclic P).
+  - assert (FF : rv = target erv) by by rewrite right_e.
+    apply (no_selfloop FF).
+Qed.
+
+Definition rem_node_graph :=
+  @add_concl_graph _ (@add_concl_graph _ rem_node_graph_1 (Sub rv rv_inside) c (flabel erv))
+                     (inl (Sub lv lv_inside)) c (flabel elv).
+
+Lemma vlabel_cv : vlabel cv = c.
+Proof. apply /eqP. by rewrite -terminal_tens_parr. Qed.
+
+Lemma v_neq_cv : v <> cv.
+Proof. intro F. have := vlabel_cv. rewrite -F. by destruct V as [V' | V']; rewrite V'. Qed.
+
+(* Give its order *)
+Definition rem_node_transport (e : edge G) : edge rem_node_graph :=
+  if @boolP _ is AltTrue p then Some (inl (Some (inl (Sub e p : edge rem_node_graph_1))))
+  else if e == elv then None else Some (inl None).
+
+Definition rem_node_order :=
+  None :: (Some (inl None)) :: [seq rem_node_transport x | x <- [seq x <- order G | x != ecv]].
+
+Definition rem_node_graph_data := {|
+  graph_of := rem_node_graph;
+  order := rem_node_order;
+  |}.
+
+Lemma rem_node_removed : edge_set (setT :\ v :\ cv) = setT :\ elv :\ erv :\ ecv.
+Proof.
+  assert (C := vlabel_cv).
+  apply /setP => a. rewrite !in_set !in_set1 !andb_true_r.
+  destruct (eq_comparable a ecv) as [? | Hc];
+  [ | destruct (eq_comparable a erv) as [? | Hr]];
+  [ | | destruct (eq_comparable a elv)];
+  try by (subst a; rewrite ?left_e ?right_e !eq_refl ?andb_false_r).
+  assert (a != ecv /\ a != erv /\ a != elv) as [-> [-> ->]] by by splitb; apply /eqP.
+  simpl. splitb; apply /eqP.
+  - by apply no_source_c.
+  - intros ?. contradict Hc. by apply ccl_eq.
+  - intros ?. contradict Hc. by apply one_target_c.
+  - intros ?. contradict Hr. by apply right_eq2.
+Qed.
+
+Definition rem_node_transport' (e : edge rem_node_graph) : edge G :=
+  match e with
+  | Some (inl (Some (inl (exist a _)))) => a
+  | Some (inl (Some (inr a)))           => match a with end
+  | Some (inl None)                     => erv
+  | Some (inr a)                        => match a with end
+  | None                                => elv
+  end.
+
+Lemma rem_node_transport'_inj : injective rem_node_transport'.
+Proof.
+  assert (elv <> erv) by apply left_neq_right.
+  move => [[[[[e E] | []] | ]| []] | ] [[[[[a A] | []] | ]| []] | ];
+  cbnb; introb; cbnb.
+  all: try by (contradict E || contradict A); apply /negP;
+    rewrite rem_node_removed // !in_set !in_set1; caseb.
+  by assert (erv <> elv) by by apply nesym.
+Qed.
+
+Lemma rem_node_transportK e :
+  e <> ecv -> rem_node_transport' (rem_node_transport e) = e.
+Proof.
+  intros ?.
+  unfold rem_node_transport, rem_node_transport'.
+  case: {-}_ /boolP => In; cbnb. case_if.
+  revert In. rewrite rem_node_removed !in_set !in_set1. introb.
+Qed.
+
+Lemma rem_node_transportK' e :
+  rem_node_transport (rem_node_transport' e) = e.
+Proof.
+  unfold rem_node_transport, rem_node_transport'.
+  destruct e as [[[[[e E] | []] | ] | []] | ];
+  case: {-}_ /boolP => In.
+  - cbnb.
+  - by contradict E; apply /negP.
+  - contradict In; apply /negP. rewrite rem_node_removed !in_set !in_set1. caseb.
+  - case_if. by assert (erv <> elv) by apply nesym, left_neq_right.
+  - contradict In; apply /negP. rewrite rem_node_removed !in_set !in_set1. caseb.
+  - by rewrite eq_refl.
+Qed.
+
+Lemma flabel_rem_node_transport' e : flabel (rem_node_transport' e) = flabel e.
+Proof. destruct e as [[[[[e E] | []] | ] | []] | ]; cbnb. Qed.
+
+Lemma rem_node_transport_in_edges_at (b : bool) (e : edge G)
+  (Hu : endpoint b e \in [set: G] :\ v :\ cv) :
+  rem_node_transport e \in edges_at_outin b (inl (inl (Sub (endpoint b e) Hu)) : rem_node_graph).
+Proof.
+  rewrite in_set /rem_node_transport.
+  case: {-}_ /boolP => In; cbnb; case_if; destruct b; cbnb.
+  - contradict Hu; apply /negP. rewrite !in_set !in_set1 left_e. caseb.
+  - revert In. rewrite rem_node_removed // !in_set !in_set1. introb.
+    all: contradict Hu; apply /negP; rewrite !in_set !in_set1 ?right_e; caseb.
+  - revert In. rewrite rem_node_removed // !in_set !in_set1. introb.
+    contradict Hu; apply /negP.
+    rewrite ccl_e !in_set !in_set1. caseb.
+Qed.
+
+Lemma rem_node_transport_edges u Hu b : edges_at_outin b u =
+  [set rem_node_transport' a | a in edges_at_outin b (inl (inl (Sub u Hu)) : rem_node_graph)].
+Proof.
+  apply /setP => e. rewrite in_set.
+  symmetry. destruct (eq_comparable u (endpoint b e)) as [? | Hc]; [subst u | ].
+  - rewrite eq_refl. apply /imsetP. exists (rem_node_transport e).
+    + apply rem_node_transport_in_edges_at.
+    + rewrite rem_node_transportK //.
+      intros ?; subst e.
+      contradict Hu; apply /negP.
+      rewrite !in_set !in_set1.
+      destruct b; rewrite ?ccl_e; caseb.
+  - transitivity false; last by by symmetry; apply /eqP; apply nesym.
+    apply /imsetP; move => [[[[[[a A] | []] | ] | []] | ] Ain /= ?]; subst e.
+    all: contradict Ain; apply /negP.
+    all: rewrite !in_set eq_sym; destruct b; cbnb; by apply /eqP.
+Qed.
+
+Lemma rem_node_p_deg : proper_degree rem_node_graph.
+Proof.
+  move => b [[[u U] | []] | []] /=.
+  - rewrite -p_deg rem_node_transport_edges card_imset //; by apply rem_node_transport'_inj.
+  - destruct b.
+    + assert (Hr : edges_at_in (inl (inr tt) : rem_node_graph) = [set Some (inl None)]).
+      { apply /setP => e; rewrite !in_set in_set1. by destruct e as [[[[[? ?] | []] | ] | []] | ]. }
+      by rewrite Hr cards1.
+    + assert (Hr : edges_at_out (inl (inr tt) : rem_node_graph) = set0).
+      { apply /setP => e; rewrite !in_set. by destruct e as [[[[[? ?] | []] | ] | []] | ]. }
+      by rewrite Hr cards0.
+  - destruct b.
+    + assert (Hr : edges_at_in (inr tt : rem_node_graph) = [set None]).
+      { apply /setP => e. rewrite !in_set in_set1. by destruct e as [[[[[? ?] | []] | ] | []] | ]. }
+      by rewrite Hr cards1.
+    + assert (Hr : edges_at_out (inr tt : rem_node_graph) = set0).
+      { apply /setP => e. rewrite !in_set. by destruct e as [[[[[? ?] | []] | ] | []] | ]. }
+      by rewrite Hr cards0.
+Qed.
+
+Lemma rem_node_p_ax_cut : proper_ax_cut rem_node_graph.
+Proof.
+  move => b [[[u U] | []] | []] /= Hu; try by destruct b.
+  destruct (p_ax_cut Hu) as [el [er [Lin [Rin LR]]]].
+  exists (rem_node_transport el), (rem_node_transport er).
+  revert Lin. rewrite rem_node_transport_edges => /imsetP[al Al ?]. subst el.
+  revert Rin. rewrite rem_node_transport_edges => /imsetP[ar Ar ?]. subst er.
+  revert LR. rewrite !flabel_rem_node_transport' => LR.
+  rewrite !rem_node_transportK'. splitb.
+Qed.
+
+Lemma rem_node_p_tens_parr : proper_tens_parr rem_node_graph.
+Proof.
+  move => b [[[u U] | []] | []] /= Hu; try by destruct b.
+  destruct (p_tens_parr Hu) as [el [er [ec [Lin [Ll [Rin [Rl [Cin Elrc]]]]]]]].
+  exists (rem_node_transport el), (rem_node_transport er), (rem_node_transport ec).
+  revert Lin. rewrite rem_node_transport_edges => /imsetP[al Al ?]. subst el.
+  revert Rin. rewrite rem_node_transport_edges => /imsetP[ar Ar ?]. subst er.
+  revert Cin. rewrite rem_node_transport_edges => /imsetP[ac Ac ?]. subst ec.
+  revert Elrc. rewrite !flabel_rem_node_transport' => Elrc.
+  rewrite !rem_node_transportK'. splitb.
+  - revert Ll. destruct al as [[[[[? ?] | []] | ] | []] | ]; cbnb.
+  - revert Rl. destruct ar as [[[[[? ?] | []] | ] | []] | ]; cbnb.
+    + contradict Ar. by rewrite !in_set.
+    + by rewrite left_l.
+Qed.
+
+Lemma rem_node_p_noleft : proper_noleft rem_node_graph.
+Proof. move => [[[[[e E] | []] | ]| []] | ] //=. by apply p_noleft. Qed.
+
+Lemma rem_node_p_order_full : proper_order_full rem_node_graph_data.
+Proof.
+  rewrite /= /rem_node_order.
+  move => [[[[[e E] | []] | ] | []] | ] //=.
+  rewrite !in_cons /=.
+  assert (Hr : Some (inl (Some (inl (Sub e E : edge rem_node_graph_1)))) = rem_node_transport e).
+  { rewrite /rem_node_transport. case: {-}_ /boolP => [In | /negP //]. cbnb. }
+  rewrite Hr {Hr}. split.
+  - move => ?. apply map_f.
+    rewrite mem_filter. splitb.
+    + revert E. rewrite rem_node_removed !in_set !in_set1. introb.
+    + by apply p_order_full.
+  - move => /mapP[a A Ha].
+    assert (a = e).
+    { revert Ha. unfold rem_node_transport. case: {-}_ /boolP => [In | /negP //].
+      case: {-}_ /boolP => [In' | /negP-? //]; last by case_if.
+      move => /eqP. by cbnb => /eqP-->. }
+    subst a.
+    revert A. rewrite mem_filter. introb.
+    by apply p_order_full.
+Qed.
+
+Lemma rem_node_p_order_uniq : proper_order_uniq rem_node_graph_data.
+Proof.
+  rewrite /proper_order_uniq /= in_cons /=. splitb.
+  - apply /mapP; move => [a A] /eqP.
+    rewrite /rem_node_transport.
+    case: {-}_ /boolP => ?; case_if.
+    revert A. rewrite mem_filter => /andP[_ A].
+    apply p_order_full in A.
+    contradict A.
+    rewrite left_e. by destruct V as [H | H]; rewrite H.
+  - apply /mapP; move => [a A] /eqP.
+    rewrite /rem_node_transport.
+    case: {-}_ /boolP => Ain; case_if.
+    revert A. rewrite mem_filter => /andP[/eqP-A0 A].
+    revert Ain. rewrite rem_node_removed // !in_set !in_set1. introb.
+    apply p_order_full in A.
+    contradict A.
+    rewrite right_e. by destruct V as [H | H]; rewrite H.
+  - rewrite map_inj_in_uniq.
+    { apply filter_uniq, p_order_uniq. }
+    intros a b.
+    rewrite !mem_filter => /andP[_ A] /andP[_ B].
+    rewrite /rem_node_transport.
+    case: {-}_ /boolP => Ain;
+    case: {-}_ /boolP => Bin => /eqP; case_if.
+    enough (L : forall e, e \notin edge_set (setT :\ v :\ cv) -> e \in order G -> e = ecv).
+    { transitivity (ccl V); [ | symmetry]; by apply L. }
+    clear - T.
+    intros a Ain A.
+    apply p_order_full in A.
+    revert Ain. rewrite rem_node_removed !in_set !in_set1. introb.
+    + contradict A. rewrite right_e. destruct V as [H | H]; by rewrite H.
+    + contradict A. rewrite left_e. destruct V as [H | H]; by rewrite H.
+Qed.
+
+Definition rem_node_ps := {|
+  graph_data_of := rem_node_graph_data;
+  p_deg := rem_node_p_deg;
+  p_ax_cut := rem_node_p_ax_cut;
+  p_tens_parr := rem_node_p_tens_parr;
+  p_noleft := rem_node_p_noleft;
+  p_order_full := rem_node_p_order_full;
+  p_order_uniq := rem_node_p_order_uniq;
+  |}.
+
+End Rem_node.
+
+
 Section Sequentializing_parr.
 Context {G : proof_net} {v : G}.
 Hypothesis (V : vlabel v = ⅋) (T : terminal v).
